Added general map comprehensions, of the form `map x,y | R(x,y) :: f(x,y) := g(x,y)`. This map takes `f(x,y)` to `g(x,y)`, where `x` and `y` are any values that satisfy `R(x, y)`. The ordinary map comprehension `map x | R(x) :: g(x)` is a special case of the general map comprehension `map x | R(x) :: x := g(x)`. Triggers have not yet been given enough thought in this design.

Source/Dafny/Cloner.cs
@@ -411,7 +411,8 @@ namespace Microsoft.Dafny
             Contract.Assert(false); throw new cce.UnreachableException();  // unexpected quantifier expression
           }
         } else if (e is MapComprehension) {
-          return new MapComprehension(tk, ((MapComprehension)e).Finite, bvs, range, term, CloneAttributes(e.Attributes));
+          var mc = (MapComprehension)e;
+          return new MapComprehension(tk, mc.Finite, bvs, range, mc.TermLeft == null ? null : CloneExpr(mc.TermLeft), term, CloneAttributes(e.Attributes));
         } else if (e is LambdaExpr) {
           var l = (LambdaExpr)e;
           return new LambdaExpr(tk, bvs, range, l.Reads.ConvertAll(CloneFrameExpr), term);
