Source/Dafny/Scanner.cs
@@ -273,50 +273,50 @@ public class Scanner {
 		for (int i = 65; i <= 90; ++i) start[i] = 1;
 		for (int i = 95; i <= 95; ++i) start[i] = 1;
 		for (int i = 99; i <= 122; ++i) start[i] = 1;
-		for (int i = 49; i <= 57; ++i) start[i] = 54;
-		start[97] = 55; 
-		start[98] = 56; 
-		start[39] = 57; 
-		start[48] = 58; 
+		for (int i = 49; i <= 57; ++i) start[i] = 55;
+		start[97] = 56; 
+		start[98] = 57; 
+		start[39] = 58; 
+		start[48] = 59; 
 		start[34] = 27; 
-		start[64] = 104; 
-		start[58] = 105; 
+		start[64] = 105; 
+		start[58] = 60; 
 		start[44] = 34; 
 		start[124] = 106; 
-		start[8226] = 37; 
+		start[8226] = 38; 
 		start[46] = 107; 
-		start[96] = 38; 
-		start[59] = 39; 
+		start[96] = 39; 
+		start[59] = 40; 
 		start[61] = 108; 
-		start[123] = 41; 
-		start[125] = 42; 
-		start[91] = 43; 
-		start[93] = 44; 
-		start[40] = 45; 
-		start[41] = 46; 
+		start[123] = 42; 
+		start[125] = 43; 
+		start[91] = 44; 
+		start[93] = 45; 
+		start[40] = 46; 
+		start[41] = 47; 
 		start[60] = 109; 
 		start[62] = 110; 
 		start[33] = 111; 
-		start[8800] = 48; 
-		start[42] = 49; 
-		start[43] = 79; 
+		start[8800] = 49; 
+		start[42] = 50; 
+		start[43] = 80; 
 		start[45] = 112; 
-		start[126] = 80; 
-		start[35] = 85; 
-		start[8804] = 87; 
-		start[8805] = 88; 
-		start[8660] = 90; 
-		start[8658] = 92; 
-		start[8656] = 93; 
+		start[126] = 81; 
+		start[35] = 86; 
+		start[8804] = 88; 
+		start[8805] = 89; 
+		start[8660] = 91; 
+		start[8658] = 93; 
+		start[8656] = 94; 
 		start[38] = 113; 
-		start[8743] = 95; 
-		start[8744] = 97; 
-		start[172] = 98; 
-		start[8704] = 99; 
-		start[8707] = 100; 
-		start[47] = 101; 
-		start[37] = 102; 
-		start[94] = 103; 
+		start[8743] = 96; 
+		start[8744] = 98; 
+		start[172] = 99; 
+		start[8704] = 100; 
+		start[8707] = 101; 
+		start[47] = 102; 
+		start[37] = 103; 
+		start[94] = 104; 
 		start[Buffer.EOF] = -1;
 
   }
@@ -535,54 +535,54 @@ public class Scanner {
 			case "seq": t.kind = 20; break;
 			case "map": t.kind = 21; break;
 			case "imap": t.kind = 22; break;
-			case "assume": t.kind = 35; break;
-			case "calc": t.kind = 36; break;
-			case "case": t.kind = 37; break;
-			case "then": t.kind = 38; break;
-			case "else": t.kind = 39; break;
-			case "as": t.kind = 40; break;
-			case "by": t.kind = 41; break;
-			case "in": t.kind = 42; break;
-			case "decreases": t.kind = 43; break;
-			case "invariant": t.kind = 44; break;
-			case "function": t.kind = 45; break;
-			case "predicate": t.kind = 46; break;
-			case "inductive": t.kind = 47; break;
-			case "twostate": t.kind = 48; break;
-			case "lemma": t.kind = 49; break;
-			case "copredicate": t.kind = 50; break;
-			case "static": t.kind = 51; break;
-			case "protected": t.kind = 52; break;
-			case "import": t.kind = 53; break;
-			case "export": t.kind = 54; break;
-			case "class": t.kind = 55; break;
-			case "trait": t.kind = 56; break;
-			case "datatype": t.kind = 57; break;
-			case "codatatype": t.kind = 58; break;
-			case "var": t.kind = 59; break;
-			case "const": t.kind = 60; break;
-			case "newtype": t.kind = 61; break;
-			case "type": t.kind = 62; break;
-			case "iterator": t.kind = 63; break;
-			case "method": t.kind = 64; break;
-			case "colemma": t.kind = 65; break;
-			case "constructor": t.kind = 66; break;
-			case "modifies": t.kind = 67; break;
-			case "reads": t.kind = 68; break;
-			case "requires": t.kind = 69; break;
-			case "ensures": t.kind = 70; break;
-			case "ghost": t.kind = 71; break;
-			case "witness": t.kind = 72; break;
-			case "reveal": t.kind = 87; break;
-			case "include": t.kind = 88; break;
-			case "abstract": t.kind = 89; break;
-			case "extern": t.kind = 90; break;
-			case "module": t.kind = 91; break;
-			case "refines": t.kind = 92; break;
-			case "opened": t.kind = 93; break;
-			case "provides": t.kind = 95; break;
-			case "reveals": t.kind = 96; break;
-			case "extends": t.kind = 97; break;
+			case "assume": t.kind = 36; break;
+			case "calc": t.kind = 37; break;
+			case "case": t.kind = 38; break;
+			case "then": t.kind = 39; break;
+			case "else": t.kind = 40; break;
+			case "as": t.kind = 41; break;
+			case "by": t.kind = 42; break;
+			case "in": t.kind = 43; break;
+			case "decreases": t.kind = 44; break;
+			case "invariant": t.kind = 45; break;
+			case "function": t.kind = 46; break;
+			case "predicate": t.kind = 47; break;
+			case "inductive": t.kind = 48; break;
+			case "twostate": t.kind = 49; break;
+			case "lemma": t.kind = 50; break;
+			case "copredicate": t.kind = 51; break;
+			case "static": t.kind = 52; break;
+			case "protected": t.kind = 53; break;
+			case "import": t.kind = 54; break;
+			case "export": t.kind = 55; break;
+			case "class": t.kind = 56; break;
+			case "trait": t.kind = 57; break;
+			case "datatype": t.kind = 58; break;
+			case "codatatype": t.kind = 59; break;
+			case "var": t.kind = 60; break;
+			case "const": t.kind = 61; break;
+			case "newtype": t.kind = 62; break;
+			case "type": t.kind = 63; break;
+			case "iterator": t.kind = 64; break;
+			case "method": t.kind = 65; break;
+			case "colemma": t.kind = 66; break;
+			case "constructor": t.kind = 67; break;
+			case "modifies": t.kind = 68; break;
+			case "reads": t.kind = 69; break;
+			case "requires": t.kind = 70; break;
+			case "ensures": t.kind = 71; break;
+			case "ghost": t.kind = 72; break;
+			case "witness": t.kind = 73; break;
+			case "reveal": t.kind = 88; break;
+			case "include": t.kind = 89; break;
+			case "abstract": t.kind = 90; break;
+			case "extern": t.kind = 91; break;
+			case "module": t.kind = 92; break;
+			case "refines": t.kind = 93; break;
+			case "opened": t.kind = 94; break;
+			case "provides": t.kind = 96; break;
+			case "reveals": t.kind = 97; break;
+			case "extends": t.kind = 98; break;
 			case "new": t.kind = 99; break;
 			case "yields": t.kind = 100; break;
 			case "returns": t.kind = 101; break;
@@ -740,7 +740,7 @@ public class Scanner {
 			case 27:
 				if (ch <= 9 || ch >= 11 && ch <= 12 || ch >= 14 && ch <= '!' || ch >= '#' && ch <= '[' || ch >= ']' && ch <= 65535) {AddCh(); goto case 27;}
 				else if (ch == '"') {AddCh(); goto case 33;}
-				else if (ch == 92) {AddCh(); goto case 61;}
+				else if (ch == 92) {AddCh(); goto case 63;}
 				else {goto case 0;}
 			case 28:
 				if (ch >= '0' && ch <= '9' || ch >= 'A' && ch <= 'F' || ch >= 'a' && ch <= 'f') {AddCh(); goto case 29;}
@@ -756,7 +756,7 @@ public class Scanner {
 				else {goto case 0;}
 			case 32:
 				if (ch <= '!' || ch >= '#' && ch <= 65535) {AddCh(); goto case 32;}
-				else if (ch == '"') {AddCh(); goto case 62;}
+				else if (ch == '"') {AddCh(); goto case 64;}
 				else {goto case 0;}
 			case 33:
 				{t.kind = 24; break;}
@@ -769,13 +769,13 @@ public class Scanner {
 			case 37:
 				{t.kind = 30; break;}
 			case 38:
-				{t.kind = 32; break;}
+				{t.kind = 31; break;}
 			case 39:
 				{t.kind = 33; break;}
 			case 40:
 				{t.kind = 34; break;}
 			case 41:
-				{t.kind = 73; break;}
+				{t.kind = 35; break;}
 			case 42:
 				{t.kind = 74; break;}
 			case 43:
@@ -787,255 +787,255 @@ public class Scanner {
 			case 46:
 				{t.kind = 78; break;}
 			case 47:
-				{t.kind = 82; break;}
+				{t.kind = 79; break;}
 			case 48:
 				{t.kind = 83; break;}
 			case 49:
 				{t.kind = 84; break;}
 			case 50:
-				if (ch == 'n') {AddCh(); goto case 51;}
-				else {goto case 0;}
+				{t.kind = 85; break;}
 			case 51:
-				if (ch <= '&' || ch >= '(' && ch <= '/' || ch >= ':' && ch <= '>' || ch == '@' || ch >= '[' && ch <= '^' || ch == '`' || ch >= '{' && ch <= 65535) {apx++; AddCh(); goto case 52;}
+				if (ch == 'n') {AddCh(); goto case 52;}
 				else {goto case 0;}
 			case 52:
+				if (ch <= '&' || ch >= '(' && ch <= '/' || ch >= ':' && ch <= '>' || ch == '@' || ch >= '[' && ch <= '^' || ch == '`' || ch >= '{' && ch <= 65535) {apx++; AddCh(); goto case 53;}
+				else {goto case 0;}
+			case 53:
 				{
 					tlen -= apx;
 					SetScannerBehindT();
-					t.kind = 85; break;}
-			case 53:
-				{t.kind = 86; break;}
+					t.kind = 86; break;}
 			case 54:
+				{t.kind = 87; break;}
+			case 55:
 				recEnd = pos; recKind = 2;
-				if (ch >= '0' && ch <= '9') {AddCh(); goto case 54;}
-				else if (ch == '_') {AddCh(); goto case 63;}
+				if (ch >= '0' && ch <= '9') {AddCh(); goto case 55;}
+				else if (ch == '_') {AddCh(); goto case 65;}
 				else if (ch == '.') {AddCh(); goto case 18;}
 				else {t.kind = 2; break;}
-			case 55:
-				recEnd = pos; recKind = 1;
-				if (ch == 39 || ch >= '0' && ch <= '9' || ch == '?' || ch >= 'A' && ch <= 'Z' || ch == '_' || ch >= 'a' && ch <= 'q' || ch >= 's' && ch <= 'z') {AddCh(); goto case 2;}
-				else if (ch == 'r') {AddCh(); goto case 64;}
-				else {t.kind = 1; t.val = new String(tval, 0, tlen); CheckLiteral(); return t;}
 			case 56:
 				recEnd = pos; recKind = 1;
-				if (ch == 39 || ch >= '0' && ch <= '9' || ch == '?' || ch >= 'A' && ch <= 'Z' || ch == '_' || ch >= 'a' && ch <= 'u' || ch >= 'w' && ch <= 'z') {AddCh(); goto case 10;}
-				else if (ch == 'v') {AddCh(); goto case 65;}
+				if (ch == 39 || ch >= '0' && ch <= '9' || ch == '?' || ch >= 'A' && ch <= 'Z' || ch == '_' || ch >= 'a' && ch <= 'q' || ch >= 's' && ch <= 'z') {AddCh(); goto case 2;}
+				else if (ch == 'r') {AddCh(); goto case 66;}
 				else {t.kind = 1; t.val = new String(tval, 0, tlen); CheckLiteral(); return t;}
 			case 57:
 				recEnd = pos; recKind = 1;
-				if (ch >= '0' && ch <= '9' || ch == '?' || ch >= 'A' && ch <= 'Z' || ch == '_' || ch >= 'a' && ch <= 'z') {AddCh(); goto case 66;}
-				else if (ch == 39) {AddCh(); goto case 67;}
-				else if (ch <= 9 || ch >= 11 && ch <= 12 || ch >= 14 && ch <= '&' || ch >= '(' && ch <= '/' || ch >= ':' && ch <= '>' || ch == '@' || ch == '[' || ch >= ']' && ch <= '^' || ch == '`' || ch >= '{' && ch <= 65535) {AddCh(); goto case 21;}
-				else if (ch == 92) {AddCh(); goto case 60;}
+				if (ch == 39 || ch >= '0' && ch <= '9' || ch == '?' || ch >= 'A' && ch <= 'Z' || ch == '_' || ch >= 'a' && ch <= 'u' || ch >= 'w' && ch <= 'z') {AddCh(); goto case 10;}
+				else if (ch == 'v') {AddCh(); goto case 67;}
 				else {t.kind = 1; t.val = new String(tval, 0, tlen); CheckLiteral(); return t;}
 			case 58:
+				recEnd = pos; recKind = 1;
+				if (ch >= '0' && ch <= '9' || ch == '?' || ch >= 'A' && ch <= 'Z' || ch == '_' || ch >= 'a' && ch <= 'z') {AddCh(); goto case 68;}
+				else if (ch == 39) {AddCh(); goto case 69;}
+				else if (ch <= 9 || ch >= 11 && ch <= 12 || ch >= 14 && ch <= '&' || ch >= '(' && ch <= '/' || ch >= ':' && ch <= '>' || ch == '@' || ch == '[' || ch >= ']' && ch <= '^' || ch == '`' || ch >= '{' && ch <= 65535) {AddCh(); goto case 21;}
+				else if (ch == 92) {AddCh(); goto case 62;}
+				else {t.kind = 1; t.val = new String(tval, 0, tlen); CheckLiteral(); return t;}
+			case 59:
 				recEnd = pos; recKind = 2;
-				if (ch >= '0' && ch <= '9') {AddCh(); goto case 54;}
-				else if (ch == '_') {AddCh(); goto case 63;}
+				if (ch >= '0' && ch <= '9') {AddCh(); goto case 55;}
+				else if (ch == '_') {AddCh(); goto case 65;}
 				else if (ch == 'x') {AddCh(); goto case 15;}
 				else if (ch == '.') {AddCh(); goto case 18;}
 				else {t.kind = 2; break;}
-			case 59:
-				recEnd = pos; recKind = 1;
-				if (ch == 39 || ch >= '0' && ch <= '9' || ch == '?' || ch >= 'A' && ch <= 'Z' || ch == '_' || ch >= 'a' && ch <= 'z') {AddCh(); goto case 59;}
-				else {t.kind = 1; t.val = new String(tval, 0, tlen); CheckLiteral(); return t;}
 			case 60:
+				recEnd = pos; recKind = 25;
+				if (ch == ':') {AddCh(); goto case 35;}
+				else if (ch == '=') {AddCh(); goto case 36;}
+				else if (ch == '|') {AddCh(); goto case 37;}
+				else {t.kind = 25; break;}
+			case 61:
+				recEnd = pos; recKind = 1;
+				if (ch == 39 || ch >= '0' && ch <= '9' || ch == '?' || ch >= 'A' && ch <= 'Z' || ch == '_' || ch >= 'a' && ch <= 'z') {AddCh(); goto case 61;}
+				else {t.kind = 1; t.val = new String(tval, 0, tlen); CheckLiteral(); return t;}
+			case 62:
 				if (ch == '"' || ch == 39 || ch == '0' || ch == 92 || ch == 'n' || ch == 'r' || ch == 't') {AddCh(); goto case 21;}
 				else if (ch == 'u') {AddCh(); goto case 22;}
 				else {goto case 0;}
-			case 61:
+			case 63:
 				if (ch == '"' || ch == 39 || ch == '0' || ch == 92 || ch == 'n' || ch == 'r' || ch == 't') {AddCh(); goto case 27;}
 				else if (ch == 'u') {AddCh(); goto case 28;}
 				else {goto case 0;}
-			case 62:
+			case 64:
 				recEnd = pos; recKind = 24;
 				if (ch == '"') {AddCh(); goto case 32;}
 				else {t.kind = 24; break;}
-			case 63:
-				if (ch >= '0' && ch <= '9') {AddCh(); goto case 54;}
-				else {goto case 0;}
-			case 64:
-				recEnd = pos; recKind = 1;
-				if (ch == 39 || ch >= '0' && ch <= '9' || ch == '?' || ch >= 'A' && ch <= 'Z' || ch == '_' || ch >= 'a' && ch <= 'q' || ch >= 's' && ch <= 'z') {AddCh(); goto case 3;}
-				else if (ch == 'r') {AddCh(); goto case 68;}
-				else {t.kind = 1; t.val = new String(tval, 0, tlen); CheckLiteral(); return t;}
 			case 65:
-				recEnd = pos; recKind = 1;
-				if (ch == 39 || ch == '?' || ch >= 'A' && ch <= 'Z' || ch == '_' || ch >= 'a' && ch <= 'z') {AddCh(); goto case 11;}
-				else if (ch >= '1' && ch <= '9') {AddCh(); goto case 69;}
-				else if (ch == '0') {AddCh(); goto case 70;}
-				else {t.kind = 1; t.val = new String(tval, 0, tlen); CheckLiteral(); return t;}
+				if (ch >= '0' && ch <= '9') {AddCh(); goto case 55;}
+				else {goto case 0;}
 			case 66:
 				recEnd = pos; recKind = 1;
-				if (ch >= '0' && ch <= '9' || ch == '?' || ch >= 'A' && ch <= 'Z' || ch == '_' || ch >= 'a' && ch <= 'z') {AddCh(); goto case 71;}
-				else if (ch == 39) {AddCh(); goto case 72;}
+				if (ch == 39 || ch >= '0' && ch <= '9' || ch == '?' || ch >= 'A' && ch <= 'Z' || ch == '_' || ch >= 'a' && ch <= 'q' || ch >= 's' && ch <= 'z') {AddCh(); goto case 3;}
+				else if (ch == 'r') {AddCh(); goto case 70;}
 				else {t.kind = 1; t.val = new String(tval, 0, tlen); CheckLiteral(); return t;}
 			case 67:
 				recEnd = pos; recKind = 1;
-				if (ch >= '0' && ch <= '9' || ch == '?' || ch >= 'A' && ch <= 'Z' || ch == '_' || ch >= 'a' && ch <= 'z') {AddCh(); goto case 71;}
-				else if (ch == 39) {AddCh(); goto case 13;}
+				if (ch == 39 || ch == '?' || ch >= 'A' && ch <= 'Z' || ch == '_' || ch >= 'a' && ch <= 'z') {AddCh(); goto case 11;}
+				else if (ch >= '1' && ch <= '9') {AddCh(); goto case 71;}
+				else if (ch == '0') {AddCh(); goto case 72;}
 				else {t.kind = 1; t.val = new String(tval, 0, tlen); CheckLiteral(); return t;}
 			case 68:
 				recEnd = pos; recKind = 1;
-				if (ch == 39 || ch >= '0' && ch <= '9' || ch == '?' || ch >= 'A' && ch <= 'Z' || ch == '_' || ch >= 'b' && ch <= 'z') {AddCh(); goto case 4;}
-				else if (ch == 'a') {AddCh(); goto case 73;}
+				if (ch >= '0' && ch <= '9' || ch == '?' || ch >= 'A' && ch <= 'Z' || ch == '_' || ch >= 'a' && ch <= 'z') {AddCh(); goto case 73;}
+				else if (ch == 39) {AddCh(); goto case 74;}
 				else {t.kind = 1; t.val = new String(tval, 0, tlen); CheckLiteral(); return t;}
 			case 69:
-				recEnd = pos; recKind = 7;
-				if (ch == 39 || ch == '?' || ch >= 'A' && ch <= 'Z' || ch == '_' || ch >= 'a' && ch <= 'z') {AddCh(); goto case 59;}
-				else if (ch >= '0' && ch <= '9') {AddCh(); goto case 69;}
-				else {t.kind = 7; break;}
+				recEnd = pos; recKind = 1;
+				if (ch >= '0' && ch <= '9' || ch == '?' || ch >= 'A' && ch <= 'Z' || ch == '_' || ch >= 'a' && ch <= 'z') {AddCh(); goto case 73;}
+				else if (ch == 39) {AddCh(); goto case 13;}
+				else {t.kind = 1; t.val = new String(tval, 0, tlen); CheckLiteral(); return t;}
 			case 70:
+				recEnd = pos; recKind = 1;
+				if (ch == 39 || ch >= '0' && ch <= '9' || ch == '?' || ch >= 'A' && ch <= 'Z' || ch == '_' || ch >= 'b' && ch <= 'z') {AddCh(); goto case 4;}
+				else if (ch == 'a') {AddCh(); goto case 75;}
+				else {t.kind = 1; t.val = new String(tval, 0, tlen); CheckLiteral(); return t;}
+			case 71:
+				recEnd = pos; recKind = 7;
+				if (ch == 39 || ch == '?' || ch >= 'A' && ch <= 'Z' || ch == '_' || ch >= 'a' && ch <= 'z') {AddCh(); goto case 61;}
+				else if (ch >= '0' && ch <= '9') {AddCh(); goto case 71;}
+				else {t.kind = 7; break;}
+			case 72:
 				recEnd = pos; recKind = 7;
 				if (ch == 39 || ch >= '0' && ch <= '9' || ch == '?' || ch >= 'A' && ch <= 'Z' || ch == '_' || ch >= 'a' && ch <= 'z') {AddCh(); goto case 12;}
 				else {t.kind = 7; break;}
-			case 71:
+			case 73:
 				recEnd = pos; recKind = 1;
 				if (ch == 39 || ch >= '0' && ch <= '9' || ch == '?' || ch >= 'A' && ch <= 'Z' || ch == '_' || ch >= 'a' && ch <= 'z') {AddCh(); goto case 14;}
 				else {t.kind = 1; t.val = new String(tval, 0, tlen); CheckLiteral(); return t;}
-			case 72:
+			case 74:
 				recEnd = pos; recKind = 23;
 				if (ch == 39 || ch >= '0' && ch <= '9' || ch == '?' || ch >= 'A' && ch <= 'Z' || ch == '_' || ch >= 'a' && ch <= 'z') {AddCh(); goto case 14;}
 				else {t.kind = 23; break;}
-			case 73:
+			case 75:
 				recEnd = pos; recKind = 1;
 				if (ch == 39 || ch >= '0' && ch <= '9' || ch == '?' || ch >= 'A' && ch <= 'Z' || ch == '_' || ch >= 'a' && ch <= 'x' || ch == 'z') {AddCh(); goto case 5;}
-				else if (ch == 'y') {AddCh(); goto case 74;}
+				else if (ch == 'y') {AddCh(); goto case 76;}
 				else {t.kind = 1; t.val = new String(tval, 0, tlen); CheckLiteral(); return t;}
-			case 74:
+			case 76:
 				recEnd = pos; recKind = 5;
 				if (ch == 39 || ch == '0' || ch >= 'A' && ch <= 'Z' || ch == '_' || ch >= 'a' && ch <= 'z') {AddCh(); goto case 6;}
-				else if (ch >= '1' && ch <= '9') {AddCh(); goto case 75;}
-				else if (ch == '?') {AddCh(); goto case 76;}
+				else if (ch >= '1' && ch <= '9') {AddCh(); goto case 77;}
+				else if (ch == '?') {AddCh(); goto case 78;}
 				else {t.kind = 5; break;}
-			case 75:
+			case 77:
 				recEnd = pos; recKind = 5;
 				if (ch == 39 || ch >= 'A' && ch <= 'Z' || ch == '_' || ch >= 'a' && ch <= 'z') {AddCh(); goto case 8;}
-				else if (ch >= '0' && ch <= '9') {AddCh(); goto case 75;}
-				else if (ch == '?') {AddCh(); goto case 77;}
+				else if (ch >= '0' && ch <= '9') {AddCh(); goto case 77;}
+				else if (ch == '?') {AddCh(); goto case 79;}
 				else {t.kind = 5; break;}
-			case 76:
+			case 78:
 				recEnd = pos; recKind = 6;
 				if (ch == 39 || ch >= '0' && ch <= '9' || ch == '?' || ch >= 'A' && ch <= 'Z' || ch == '_' || ch >= 'a' && ch <= 'z') {AddCh(); goto case 7;}
 				else {t.kind = 6; break;}
-			case 77:
+			case 79:
 				recEnd = pos; recKind = 6;
 				if (ch == 39 || ch >= '0' && ch <= '9' || ch == '?' || ch >= 'A' && ch <= 'Z' || ch == '_' || ch >= 'a' && ch <= 'z') {AddCh(); goto case 9;}
 				else {t.kind = 6; break;}
-			case 78:
-				{t.kind = 98; break;}
-			case 79:
-				{t.kind = 102; break;}
 			case 80:
-				if (ch == '>') {AddCh(); goto case 81;}
-				else {goto case 0;}
+				{t.kind = 102; break;}
 			case 81:
-				{t.kind = 108; break;}
-			case 82:
-				if (ch == '>') {AddCh(); goto case 83;}
+				if (ch == '>') {AddCh(); goto case 82;}
 				else {goto case 0;}
+			case 82:
+				{t.kind = 108; break;}
 			case 83:
-				{t.kind = 109; break;}
+				if (ch == '>') {AddCh(); goto case 84;}
+				else {goto case 0;}
 			case 84:
-				{t.kind = 110; break;}
+				{t.kind = 109; break;}
 			case 85:
-				{t.kind = 123; break;}
+				{t.kind = 110; break;}
 			case 86:
-				{t.kind = 125; break;}
+				{t.kind = 123; break;}
 			case 87:
-				{t.kind = 126; break;}
+				{t.kind = 125; break;}
 			case 88:
-				{t.kind = 127; break;}
+				{t.kind = 126; break;}
 			case 89:
-				{t.kind = 128; break;}
+				{t.kind = 127; break;}
 			case 90:
-				{t.kind = 129; break;}
+				{t.kind = 128; break;}
 			case 91:
-				{t.kind = 130; break;}
+				{t.kind = 129; break;}
 			case 92:
-				{t.kind = 131; break;}
+				{t.kind = 130; break;}
 			case 93:
-				{t.kind = 133; break;}
+				{t.kind = 131; break;}
 			case 94:
-				{t.kind = 134; break;}
+				{t.kind = 133; break;}
 			case 95:
-				{t.kind = 135; break;}
+				{t.kind = 134; break;}
 			case 96:
-				{t.kind = 136; break;}
+				{t.kind = 135; break;}
 			case 97:
-				{t.kind = 137; break;}
+				{t.kind = 136; break;}
 			case 98:
-				{t.kind = 138; break;}
+				{t.kind = 137; break;}
 			case 99:
-				{t.kind = 139; break;}
+				{t.kind = 138; break;}
 			case 100:
-				{t.kind = 141; break;}
+				{t.kind = 139; break;}
 			case 101:
-				{t.kind = 142; break;}
+				{t.kind = 141; break;}
 			case 102:
-				{t.kind = 143; break;}
+				{t.kind = 142; break;}
 			case 103:
-				{t.kind = 145; break;}
+				{t.kind = 143; break;}
 			case 104:
+				{t.kind = 145; break;}
+			case 105:
 				recEnd = pos; recKind = 153;
 				if (ch == '"') {AddCh(); goto case 32;}
 				else {t.kind = 153; break;}
-			case 105:
-				recEnd = pos; recKind = 25;
-				if (ch == ':') {AddCh(); goto case 35;}
-				else if (ch == '|') {AddCh(); goto case 36;}
-				else if (ch == '=') {AddCh(); goto case 78;}
-				else {t.kind = 25; break;}
 			case 106:
 				recEnd = pos; recKind = 27;
-				if (ch == '|') {AddCh(); goto case 96;}
+				if (ch == '|') {AddCh(); goto case 97;}
 				else {t.kind = 27; break;}
 			case 107:
-				recEnd = pos; recKind = 31;
+				recEnd = pos; recKind = 32;
 				if (ch == '.') {AddCh(); goto case 114;}
-				else {t.kind = 31; break;}
+				else {t.kind = 32; break;}
 			case 108:
-				recEnd = pos; recKind = 94;
-				if (ch == '>') {AddCh(); goto case 40;}
+				recEnd = pos; recKind = 95;
+				if (ch == '>') {AddCh(); goto case 41;}
 				else if (ch == '=') {AddCh(); goto case 115;}
-				else {t.kind = 94; break;}
+				else {t.kind = 95; break;}
 			case 109:
-				recEnd = pos; recKind = 79;
-				if (ch == '=') {AddCh(); goto case 116;}
-				else {t.kind = 79; break;}
-			case 110:
 				recEnd = pos; recKind = 80;
-				if (ch == '=') {AddCh(); goto case 86;}
+				if (ch == '=') {AddCh(); goto case 116;}
 				else {t.kind = 80; break;}
+			case 110:
+				recEnd = pos; recKind = 81;
+				if (ch == '=') {AddCh(); goto case 87;}
+				else {t.kind = 81; break;}
 			case 111:
 				recEnd = pos; recKind = 103;
-				if (ch == '=') {AddCh(); goto case 47;}
-				else if (ch == 'i') {AddCh(); goto case 50;}
+				if (ch == '=') {AddCh(); goto case 48;}
+				else if (ch == 'i') {AddCh(); goto case 51;}
 				else {t.kind = 103; break;}
 			case 112:
 				recEnd = pos; recKind = 104;
-				if (ch == '-') {AddCh(); goto case 82;}
-				else if (ch == '>') {AddCh(); goto case 84;}
+				if (ch == '-') {AddCh(); goto case 83;}
+				else if (ch == '>') {AddCh(); goto case 85;}
 				else {t.kind = 104; break;}
 			case 113:
 				recEnd = pos; recKind = 144;
-				if (ch == '&') {AddCh(); goto case 94;}
+				if (ch == '&') {AddCh(); goto case 95;}
 				else {t.kind = 144; break;}
 			case 114:
 				recEnd = pos; recKind = 155;
-				if (ch == '.') {AddCh(); goto case 53;}
+				if (ch == '.') {AddCh(); goto case 54;}
 				else {t.kind = 155; break;}
 			case 115:
-				recEnd = pos; recKind = 81;
-				if (ch == '>') {AddCh(); goto case 91;}
-				else {t.kind = 81; break;}
+				recEnd = pos; recKind = 82;
+				if (ch == '>') {AddCh(); goto case 92;}
+				else {t.kind = 82; break;}
 			case 116:
 				recEnd = pos; recKind = 124;
 				if (ch == '=') {AddCh(); goto case 117;}
 				else {t.kind = 124; break;}
 			case 117:
 				recEnd = pos; recKind = 132;
-				if (ch == '>') {AddCh(); goto case 89;}
+				if (ch == '>') {AddCh(); goto case 90;}
 				else {t.kind = 132; break;}
 
     }
