Test/dafny0/Maps.dfy
@@ -194,3 +194,52 @@ method m15(b: set<A>)
   var aa := new A;
   assert aa !in m;
 }
+
+function method Plus(x: int, y: int): int { x + y }  // a symbol to appear in trigger
+method GeneralMaps0() {
+  var m := map x | 2 <= x < 6 :: x+1;
+  assert 5 in m.Keys;
+  assert 6 !in m.Keys;
+  assert m[5] == 6;
+  assert 6 in m.Values;
+  assert (5,6) in m.Items;
+  m := map y | 2 <= y < 6 :: Plus(y, 1) := y + 3;
+  assert Plus(5, 1) in m.Keys;
+  assert 7 !in m.Keys;
+  assert m[6] == 8;
+  assert 8 in m.Values;
+  assert (6,8) in m.Items;
+}
+
+function method f(x: int): int  // uninterpreted function
+  requires 0 <= x
+function method g(x: int): int  // uninterpreted function
+
+method GeneralMaps1() {
+  if * {
+    var m := map z | 2 <= z < 6 :: z/2 := z;  // error: LHSs not unique
+  } else if * {
+    var m := map z | 2 <= z < 6 :: z/2 := z/2 + 3;  // fine, since corresponding RHSs are the same
+  } else if * {
+    var m := map z | 2 <= z < 6 :: f(z) := 20;  // fine, since corresponding RHSs are the same
+  } else if * {
+    var m := map z | 2 <= z < 6 :: f(z) := z;  // error: LHSs not (known to be) unique
+  }
+}
+
+ghost method GeneralMaps2() {
+  if * {
+    var m := imap z | 2 <= z < 6 :: g(z) := z;  // error: LHSs not (known to be) unique
+  } else {
+    var m := imap z :: g(z) := z;  // error: LHSs not (known to be) unique
+  }
+}
+
+method GeneralMaps3() {
+  // well-formedness
+  if * {
+    var m := map u | -2 <= u < 6 :: u := f(u);  // error: RHS may not be defined
+  } else if * {
+    var m := map u | -2 <= u < 6 :: f(u) := u;  // error: LHS may not be defined (also, LHS non-unique)
+  }
+}
